theories/program_logic/total_weakestpre.v
@@ -10,10 +10,10 @@ Definition twp_pre `{irisG Λ Σ} (s : stuckness)
   match to_val e1 with
   | Some v => |={E}=> Φ v
   | None => ∀ σ1 κs,
-     state_interp σ1 κs ={E,∅}=∗ ⌜if s is NotStuck then reducible e1 σ1 else True⌝ ∗
-     ∀ κ κs' e2 σ2 efs, ⌜prim_step e1 σ1 κ e2 σ2 efs ∧ κs = cons_obs κ κs'⌝ ={∅,E}=∗
-       state_interp σ2 κs' ∗ wp E e2 Φ ∗
-       [∗ list] ef ∈ efs, wp ⊤ ef (λ _, True)
+     state_interp σ1 κs ={E,∅}=∗ ⌜if s is NotStuck then reducible_no_obs e1 σ1 else True⌝ ∗
+     ∀ κ e2 σ2 efs, ⌜prim_step e1 σ1 κ e2 σ2 efs⌝ ={∅,E}=∗
+       ⌜κ = None⌝ ∗ state_interp σ2 κs ∗
+       wp E e2 Φ ∗ [∗ list] ef ∈ efs, wp ⊤ ef (λ _, True)
   end%I.
 
 Lemma twp_pre_mono `{irisG Λ Σ} s
@@ -24,8 +24,9 @@ Proof.
   iIntros "#H"; iIntros (E e1 Φ) "Hwp". rewrite /twp_pre.
   destruct (to_val e1) as [v|]; first done.
   iIntros (σ1 κs) "Hσ". iMod ("Hwp" with "Hσ") as "($ & Hwp)"; iModIntro.
-  iIntros (κ κs' e2 σ2 efs) "Hstep".
-  iMod ("Hwp" with "Hstep") as "($ & Hwp & Hfork)"; iModIntro; iSplitL "Hwp".
+  iIntros (κ e2 σ2 efs) "Hstep".
+  iMod ("Hwp" with "Hstep") as "($ & $ & Hwp & Hfork)"; iModIntro.
+  iSplitL "Hwp".
   - by iApply "H".
   - iApply (@big_sepL_impl with "[$Hfork]"); iIntros "!#" (k e _) "Hwp".
     by iApply "H".
@@ -44,7 +45,7 @@ Proof.
     iApply twp_pre_mono. iIntros "!#" (E e Φ). iApply ("H" $! (E,e,Φ)).
   - intros wp Hwp n [[E1 e1] Φ1] [[E2 e2] Φ2]
       [[?%leibniz_equiv ?%leibniz_equiv] ?]; simplify_eq/=.
-    rewrite /uncurry3 /twp_pre. do 22 (f_equiv || done). by apply Hwp, pair_ne.
+    rewrite /uncurry3 /twp_pre. do 22 (f_equiv || done). by apply pair_ne.
 Qed.
 
 Definition twp_def `{irisG Λ Σ} (s : stuckness) (E : coPset)
@@ -107,8 +108,8 @@ Proof.
   { iApply ("HΦ" with "[> -]"). by iApply (fupd_mask_mono E1 _). }
   iIntros (σ1 κs) "Hσ". iMod (fupd_intro_mask' E2 E1) as "Hclose"; first done.
   iMod ("IH" with "[$]") as "[% IH]".
-  iModIntro; iSplit; [by destruct s1, s2|]. iIntros (κ κs' e2 σ2 efs Hstep).
-  iMod ("IH" with "[//]") as "($ & IH & IHefs)"; auto.
+  iModIntro; iSplit; [by destruct s1, s2|]. iIntros (κ e2 σ2 efs Hstep).
+  iMod ("IH" with "[//]") as "($ & $ & IH & IHefs)"; auto.
   iMod "Hclose" as "_"; iModIntro. iSplitR "IHefs".
   - iDestruct "IH" as "[IH _]". iApply ("IH" with "[//] HΦ").
   - iApply (big_sepL_impl with "[$IHefs]"); iIntros "!#" (k ef _) "[IH _]".
@@ -131,14 +132,15 @@ Proof.
   destruct (to_val e) as [v|] eqn:He.
   { by iDestruct "H" as ">>> $". }
   iIntros (σ1 κs) "Hσ". iMod "H". iMod ("H" $! σ1 with "Hσ") as "[$ H]".
-  iModIntro. iIntros (κ κs' e2 σ2 efs [Hstep ->]).
-  iMod ("H" with "[//]") as "(Hphy & H & $)". destruct s.
+  iModIntro. iIntros (κ e2 σ2 efs Hstep).
+  iMod ("H" with "[//]") as "(% & Hphy & H & $)". destruct s.
   - rewrite !twp_unfold /twp_pre. destruct (to_val e2) as [v2|] eqn:He2.
     + iDestruct "H" as ">> $". by iFrame.
-    + iMod ("H" with "[$]") as "[H _]". iDestruct "H" as %(? & ? & ? & ? & ?).
+    + iMod ("H" with "[$]") as "[H _]". iDestruct "H" as %(? & ? & ? & ?).
       by edestruct (atomic _ _ _ _ _ Hstep).
   - destruct (atomic _ _ _ _ _ Hstep) as [v <-%of_to_val].
-    iMod (twp_value_inv' with "H") as ">H". iFrame "Hphy". by iApply twp_value'.
+    iMod (twp_value_inv' with "H") as ">H". iModIntro. iSplit; first done.
+    iFrame "Hphy". by iApply twp_value'.
 Qed.
 
 Lemma twp_bind K `{!LanguageCtx K} s E e Φ :
@@ -153,11 +155,11 @@ Proof.
   { apply of_to_val in He as <-. iApply fupd_twp. by iApply "HΦ". }
   rewrite twp_unfold /twp_pre fill_not_val //.
   iIntros (σ1 κs) "Hσ". iMod ("IH" with "[$]") as "[% IH]". iModIntro; iSplit.
-  { iPureIntro. unfold reducible in *.
+  { iPureIntro. unfold reducible_no_obs in *.
     destruct s; naive_solver eauto using fill_step. }
-  iIntros (κ κs' e2 σ2 efs [Hstep ->]).
+  iIntros (κ e2 σ2 efs Hstep).
   destruct (fill_step_inv e σ1 κ e2 σ2 efs) as (e2'&->&?); auto.
-  iMod ("IH" $! κ κs' e2' σ2 efs with "[//]") as "($ & IH & IHfork)".
+  iMod ("IH" $! κ e2' σ2 efs with "[//]") as "($ & $ & IH & IHfork)".
   iModIntro; iSplitR "IHfork".
   - iDestruct "IH" as "[IH _]". by iApply "IH".
   - by setoid_rewrite and_elim_r.
@@ -174,9 +176,9 @@ Proof.
     iApply (twp_pre_mono with "[] IH"). by iIntros "!#" (E e Φ') "[_ ?]". }
   rewrite /twp_pre fill_not_val //.
   iIntros (σ1 κs) "Hσ". iMod ("IH" with "[$]") as "[% IH]". iModIntro; iSplit.
-  { destruct s; eauto using reducible_fill. }
-  iIntros (κ κs' e2 σ2 efs [Hstep ->]).
-  iMod ("IH" $! κ κs' (K e2) σ2 efs with "[]") as "($ & IH & IHfork)"; eauto using fill_step.
+  { destruct s; eauto using reducible_no_obs_fill. }
+  iIntros (κ e2 σ2 efs Hstep).
+  iMod ("IH" $! κ (K e2) σ2 efs with "[]") as "($ & $ & IH & IHfork)"; eauto using fill_step.
   iModIntro; iSplitR "IHfork".
   - iDestruct "IH" as "[IH _]". by iApply "IH".
   - by setoid_rewrite and_elim_r.
@@ -186,8 +188,10 @@ Lemma twp_wp s E e Φ : WP e @ s; E [{ Φ }] -∗ WP e @ s; E {{ Φ }}.
 Proof.
   iIntros "H". iLöb as "IH" forall (E e Φ).
   rewrite wp_unfold twp_unfold /wp_pre /twp_pre. destruct (to_val e) as [v|]=>//.
-  iIntros (σ1 κs) "Hσ". iMod ("H" with "Hσ") as "[$ H]". iIntros "!>".
-  iIntros (κ κs' e2 σ2 efs) "Hstep". iMod ("H" with "Hstep") as "($ & H & Hfork)".
+  iIntros (σ1 κs) "Hσ". iMod ("H" with "Hσ") as "[% H]". iIntros "!>". iSplitR.
+  { destruct s; last done. eauto using reducible_no_obs_reducible. }
+  iIntros (κ κs' e2 σ2 efs [Hstep ->]). iMod ("H" $! _ _ _ _ Hstep) as "(% & Hst & H & Hfork)".
+  subst κ. iFrame "Hst".
   iApply step_fupd_intro; [set_solver+|]. iNext.
   iSplitL "H". by iApply "IH". iApply (@big_sepL_impl with "[$Hfork]").
   iIntros "!#" (k e' _) "H". by iApply "IH".
