theories/program_logic/total_lifting.v
@@ -14,28 +14,29 @@ Implicit Types Φ : val Λ → iProp Σ.
 Lemma twp_lift_step s E Φ e1 :
   to_val e1 = None →
   (∀ σ1 κs, state_interp σ1 κs ={E,∅}=∗
-    ⌜if s is NotStuck then reducible e1 σ1 else True⌝ ∗
-    ∀ κ κs' e2 σ2 efs, ⌜prim_step e1 σ1 κ e2 σ2 efs ∧ κs = cons_obs κ κs'⌝ ={∅,E}=∗
-      state_interp σ2 κs' ∗ WP e2 @ s; E [{ Φ }] ∗ [∗ list] ef ∈ efs, WP ef @ s; ⊤ [{ _, True }])
+    ⌜if s is NotStuck then reducible_no_obs e1 σ1 else True⌝ ∗
+    ∀ κ e2 σ2 efs, ⌜prim_step e1 σ1 κ e2 σ2 efs⌝ ={∅,E}=∗
+      ⌜κ = None⌝ ∗ state_interp σ2 κs ∗ WP e2 @ s; E [{ Φ }] ∗ [∗ list] ef ∈ efs, WP ef @ s; ⊤ [{ _, True }])
   ⊢ WP e1 @ s; E [{ Φ }].
 Proof. by rewrite twp_unfold /twp_pre=> ->. Qed.
 
 (** Derived lifting lemmas. *)
 
 Lemma twp_lift_pure_step `{Inhabited (state Λ)} s E Φ e1 :
-  (∀ σ1, reducible e1 σ1) →
+  (∀ σ1, reducible_no_obs e1 σ1) →
   (∀ σ1 κ e2 σ2 efs, prim_step e1 σ1 κ e2 σ2 efs → κ = None /\ σ1 = σ2) →
   (|={E}=> ∀ κ e2 efs σ, ⌜prim_step e1 σ κ e2 σ efs⌝ →
     WP e2 @ s; E [{ Φ }] ∗ [∗ list] ef ∈ efs, WP ef @ s; ⊤ [{ _, True }])
   ⊢ WP e1 @ s; E [{ Φ }].
 Proof.
   iIntros (Hsafe Hstep) "H". iApply twp_lift_step.
-  { eapply reducible_not_val, (Hsafe inhabitant). }
+  { eapply reducible_not_val, reducible_no_obs_reducible, (Hsafe inhabitant). }
   iIntros (σ1 κs) "Hσ". iMod "H".
   iMod fupd_intro_mask' as "Hclose"; last iModIntro; first set_solver.
-  iSplit; [by destruct s|]; iIntros (κ κs' e2 σ2 efs [Hstep' ->]).
+  iSplit; [by destruct s|]. iIntros (κ e2 σ2 efs Hstep').
   destruct (Hstep σ1 κ e2 σ2 efs); auto; subst.
-  iMod "Hclose" as "_". iFrame "Hσ". iApply "H"; auto.
+  iMod "Hclose" as "_". iModIntro. iSplit; first done.
+  iFrame "Hσ". iApply "H"; auto.
 Qed.
 
 (* Atomic steps don't need any mask-changing business here, one can
@@ -43,23 +44,23 @@ Qed.
 Lemma twp_lift_atomic_step {s E Φ} e1 :
   to_val e1 = None →
   (∀ σ1 κs, state_interp σ1 κs ={E}=∗
-    ⌜if s is NotStuck then reducible e1 σ1 else True⌝ ∗
-    ∀ κ κs' e2 σ2 efs, ⌜prim_step e1 σ1 κ e2 σ2 efs ∧ κs = cons_obs κ κs'⌝ ={E}=∗
-      state_interp σ2 κs' ∗
+    ⌜if s is NotStuck then reducible_no_obs e1 σ1 else True⌝ ∗
+    ∀ κ e2 σ2 efs, ⌜prim_step e1 σ1 κ e2 σ2 efs⌝ ={E}=∗
+      ⌜κ = None⌝ ∗ state_interp σ2 κs ∗
       from_option Φ False (to_val e2) ∗ [∗ list] ef ∈ efs, WP ef @ s; ⊤ [{ _, True }])
   ⊢ WP e1 @ s; E [{ Φ }].
 Proof.
   iIntros (?) "H". iApply (twp_lift_step _ E _ e1)=>//; iIntros (σ1 κs) "Hσ1".
   iMod ("H" $! σ1 with "Hσ1") as "[$ H]".
   iMod (fupd_intro_mask' E ∅) as "Hclose"; first set_solver.
-  iIntros "!>" (κ κs' e2 σ2 efs) "%". iMod "Hclose" as "_".
-  iMod ("H" $! κ κs' e2 σ2 efs with "[#]") as "($ & HΦ & $)"; first by eauto.
+  iIntros "!>" (κ e2 σ2 efs) "%". iMod "Hclose" as "_".
+  iMod ("H" $! κ e2 σ2 efs with "[#]") as "($ & $ & HΦ & $)"; first by eauto.
   destruct (to_val e2) eqn:?; last by iExFalso.
   iApply twp_value; last done. by apply of_to_val.
 Qed.
 
 Lemma twp_lift_pure_det_step `{Inhabited (state Λ)} {s E Φ} e1 e2 efs :
-  (∀ σ1, reducible e1 σ1) →
+  (∀ σ1, reducible_no_obs e1 σ1) →
   (∀ σ1 κ e2' σ2 efs', prim_step e1 σ1 κ e2' σ2 efs' → κ = None /\ σ1 = σ2 ∧ e2 = e2' ∧ efs = efs')→
   (|={E}=> WP e2 @ s; E [{ Φ }] ∗ [∗ list] ef ∈ efs, WP ef @ s; ⊤ [{ _, True }])
   ⊢ WP e1 @ s; E [{ Φ }].
